Examples/Scroll/Keccak/Soundness/Sequencing/Final.lean
@@ -1,0 +1,8 @@
+import Examples.Scroll.Keccak.Spec.Program
+
+namespace Keccak.Soundness
+
+  -- meets_constraints →
+  --   ∃ input_bytes, output_bytes, data_rlc c 300 = rlc input_bytes ∧ hash_rlc c 300 = rlc output_bytes
+
+end Keccak.Soundness
